Test/dafny0/Datatypes.dfy
@@ -4,12 +4,12 @@
 datatype List<T> = Nil | Cons(T, List<T>)
 
 class Node {
-  var data: int;
-  var next: Node?;
+  var data: int
+  var next: Node?
 
   function Repr(list: List<int>): bool
-    reads *;
-    decreases list;
+    reads *
+    decreases list
   { match list
     case Nil =>
       next == null
@@ -18,15 +18,15 @@ class Node {
   }
 
   method Init()
-    modifies this;
-    ensures Repr(Nil);
+		modifies this
+    ensures Repr(Nil)
   {
     next := null;
   }
 
   method Add(d: int, L: List<int>) returns (r: Node)
-    requires Repr(L);
-    ensures r != null && r.Repr(Cons(d, L));
+    requires Repr(L)
+    ensures r.Repr(Cons(d, L))
   {
     r := new Node;
     r.data := d;
@@ -35,12 +35,12 @@ class Node {
 }
 
 class AnotherNode {
-  var data: int;
-  var next: AnotherNode?;
+  var data: int
+  var next: AnotherNode?
 
-  function Repr(n: AnotherNode?, list: List<int>): bool
-    reads *;
-    decreases list;
+  predicate Repr(n: AnotherNode?, list: List<int>)
+    reads *
+    decreases list
   { match list
     case Nil =>
       n == null
@@ -49,14 +49,14 @@ class AnotherNode {
   }
 
   method Create() returns (n: AnotherNode?)
-    ensures Repr(n, Nil);
+    ensures Repr(n, Nil)
   {
     n := null;
   }
 
   method Add(n: AnotherNode, d: int, L: List<int>) returns (r: AnotherNode)
-    requires Repr(n, L);
-    ensures Repr(r, Cons(d, L));
+    requires Repr(n, L)
+    ensures Repr(r, Cons(d, L))
   {
     r := new AnotherNode;
     r.data := d;
